src/tpcms/heap.v
@@ -1,0 +1,185 @@
+Require Import Burrow.rollup.
+From stdpp Require Import gmap.
+
+Require Import Burrow.CpdtTactics.
+Require Import coq_tricks.Deex.
+
+Require Import Tpcms.auth_frag.
+Require Import Tpcms.gmap.
+
+Definition HeapT P V `{!EqDecision V} `{!EqDecision P} `{!Countable P} :=
+    AuthFrag (gmap P (option V)).
+    
+Definition map_somes {P} {V} `{Countable P} (σ : gmap P V) : gmap P (option V)
+  := fmap Some σ.
+
+Lemma lookup_map_somes {P} {V} `{Countable P} (σ : gmap P V) k
+  : map_somes σ !! k = match σ !! k with Some x => Some (Some x) | None => None end.
+Proof.
+  unfold map_somes. rewrite lookup_fmap. unfold "<$>", option_fmap, option_map. trivial.
+Qed.
+
+Lemma map_somes_insert {P} {V} `{Countable P} (σ: gmap P V) l v
+  : map_somes (<[ l := v ]> σ) = <[ l := Some v ]> (map_somes σ).
+  Admitted.
+ 
+
+Section HeapT.
+
+Context P V `{!EqDecision V} `{!EqDecision P} `{!Countable P}.
+  
+Lemma heapt_alloc (m : gmap P (option V)) (l: P) (v: V)
+  : m !! l = None →
+  mov (auth m) (dot (auth ((<[l:= Some v]> m))) (frag ({[l := Some v]} : gmap P (option V)))).
+Proof. intro.
+  unfold mov, auth, frag, af_tpcm, af_mov. intros. unfold af_dot.
+  unfold dot, gmap_tpcm. destruct z.
+  unfold af_valid in *.
+  unfold auth_dot in *.
+  unfold af_dot in *.
+  unfold auth_dot in *.
+  unfold m_valid, gmap_tpcm, gmap_valid in H0.
+  destruct o.
+  - trivial.
+  - destruct_ands. deex. split.
+    + unfold m_valid, gmap_valid. intro.
+      have h : Decision (k = l) by solve_decision. destruct h.
+      * subst k. rewrite lookup_insert. trivial.
+      * rewrite lookup_insert_ne.
+        -- have q := H0 k. destruct (m !! k); trivial.
+        -- intuition.
+    + exists c.
+      rewrite unit_dot_left in H1.
+      subst m.
+      rewrite <- gmap_dot_assoc.
+      unfold dot in *. unfold gmap_dot, unit in *.
+      apply map_eq. intro.
+      unfold gmerge in *.
+      have q := H0 i. clear H0.
+      have h : Decision (i = l) by solve_decision. destruct h.
+      * subst i. rewrite lookup_insert.
+          rewrite lookup_merge. unfold diag_None.
+          rewrite lookup_merge. unfold diag_None.
+          rewrite lookup_merge. unfold diag_None.
+          rewrite lookup_merge in q. unfold diag_None in q.
+          rewrite lookup_merge in H. unfold diag_None in H.
+          rewrite lookup_singleton.
+          rewrite lookup_empty.
+          destruct (c !! l), (g !! l); intuition.
+          -- discriminate.
+          -- discriminate.
+      * rewrite lookup_insert_ne.
+        -- rewrite lookup_merge. unfold diag_None.
+           rewrite lookup_merge. unfold diag_None.
+           rewrite lookup_merge. unfold diag_None.
+           rewrite lookup_merge. unfold diag_None.
+           rewrite lookup_merge in q. unfold diag_None in q.
+           rewrite lookup_merge in H. unfold diag_None in H.
+           rewrite lookup_singleton_ne; trivial.
+           rewrite lookup_empty.
+           destruct (c !! i), (g !! i); intuition.
+           crush.
+        -- crush.
+Qed.
+
+Lemma auth_frag_agree' (l: P) (v: V) (m: gmap P (option V))
+  (va : m_valid (dot (auth m) (frag ({[l := Some v]} : gmap P (option V)))))
+  : m !! l = Some (Some v).
+Proof.
+  unfold m_valid, af_tpcm, af_valid, dot, gmap_tpcm, af_dot, auth, frag,
+      auth_dot, gmap_dot in va. destruct_ands. deex.
+  rewrite unit_dot_left in H0.
+  subst m.
+  rewrite lookup_merge. unfold diag_None. rewrite lookup_singleton.
+  unfold m_valid, gmap_valid in H. have h := H l. clear H.
+  rewrite lookup_merge in h. unfold diag_None in h. rewrite lookup_singleton in h.
+  unfold gmerge in h. destruct (c !! l).
+  - contradiction.
+  - unfold gmerge. trivial.
+Qed.
+
+Lemma auth_frag_agree (l: P) (v: V) (m: gmap P V)
+  (va : m_valid (dot (auth (map_somes m)) (frag ({[l := Some v]} : gmap P (option V)))))
+  : m !! l = Some v.
+Proof.
+  have h := auth_frag_agree' l v (map_somes m) va.
+  unfold map_somes. rewrite lookup_fmap in h. unfold "<$>" in h.
+  unfold option_fmap, option_map in h. destruct (m !! l); crush.
+Qed.
+
+Lemma auth_frag_update' (l: P) (v1 v2: V) (m: gmap P (option V))
+  (va : m !! l = Some (Some v1))
+  : mov (dot (auth m) (frag {[l := Some v1]}))
+    (dot (auth (<[l := Some v2]> m)) (frag {[l := Some v2]})).
+(*
+Proof.
+  unfold mov, af_tpcm, af_mov. intro. unfold af_valid, af_dot, dot, gmap_tpcm,
+      auth, frag. destruct z. unfold auth_dot.
+  unfold m_valid, gmap_valid, gmap_dot. destruct o.
+  - intuition.
+  - intros. destruct_ands. deex. split.
+    + intro. have h := H k. clear H.
+      have ed : Decision (k = l) by solve_decision. destruct ed.
+      * subst l. rewrite lookup_insert. trivial.
+      * rewrite lookup_insert_ne; trivial. crush.
+    + exists c.
+      subst m.
+      apply map_eq. intro k. have h := H k. clear H.
+      have ed : Decision (k = l) by solve_decision. destruct ed.
+      * subst l. rewrite lookup_insert. unfold gmerge in *.
+        rewrite lookup_merge. unfold diag_None.
+        rewrite lookup_merge. unfold diag_None.
+        rewrite lookup_merge. unfold diag_None.
+        rewrite lookup_singleton.
+        unfold unit.
+        rewrite lookup_empty.
+        rewrite lookup_merge in h. unfold diag_None in h.
+        rewrite lookup_merge in h. unfold diag_None in h.
+        rewrite lookup_merge in h. unfold diag_None in h.
+        rewrite lookup_singleton in h.
+        unfold unit in h.
+        rewrite lookup_empty in h.
+        destruct (g !! k), (c !! k); trivial; contradiction.
+      * assert (l ≠ k) by crush.
+        unfold gmerge.
+        rewrite lookup_insert_ne; trivial.
+        rewrite lookup_merge. unfold diag_None.
+        rewrite lookup_merge. unfold diag_None.
+        rewrite lookup_merge. unfold diag_None.
+        rewrite lookup_merge. unfold diag_None.
+        rewrite lookup_merge. unfold diag_None.
+        rewrite lookup_merge. unfold diag_None.
+        unfold unit. rewrite lookup_empty.
+        rewrite lookup_singleton_ne; trivial.
+        rewrite lookup_singleton_ne; trivial.
+Qed. *) (* long Qed *)
+Admitted.
+
+Lemma auth_frag_update (l: P) (v1 v2: V) (σ: gmap P V)
+  (va : σ !! l = Some v1)
+  : mov (dot (auth (map_somes σ)) (frag {[l := Some v1]}))
+    (dot (auth (map_somes (<[l:=v2]> σ))) (frag {[l := Some v2]})).
+Proof.
+  rewrite map_somes_insert.
+  have j := auth_frag_update' l v1 v2 (map_somes σ). apply j.
+  unfold map_somes. rewrite lookup_fmap. unfold "<$>".
+  unfold option_fmap, option_map. destruct (σ !! l); crush.
+Qed.
+
+Lemma auth_empty_valid
+  : m_valid (auth (∅ : gmap P (option V))).
+Proof. unfold m_valid, af_tpcm, af_valid, auth. split.
+  - replace ((∅ : gmap P (option V))) with (unit : gmap P (option V)).
+    apply unit_valid. trivial.
+  - exists (unit : gmap P (option V)). rewrite unit_dot. trivial.
+Qed.
+
+Lemma auth_map_somes (σ : gmap P V)
+  : m_valid (auth (map_somes σ)).
+Proof. unfold m_valid, af_tpcm, af_valid, auth. split.
+  - unfold m_valid, gmap_tpcm. unfold gmap_valid. intro. 
+    rewrite lookup_map_somes. destruct (σ !! k); trivial.
+  - exists (map_somes σ). rewrite unit_dot_left. trivial.
+Qed.
+
+End HeapT.
